PiLL/PiLL/Examples.lean
@@ -1,0 +1,33 @@
+import PiLL.Definitions
+
+---------------------------------------- EXAMPLES ----------------------------------------
+
+-- Latch_xyz example from main.pdf
+-- TODO: Try and use simp more, try and omit giving explicit types to cut,
+--       in general try minimizing things given to cut
+example (x x₁ x₂ y y₁ y₂ z : PName) :
+  ⊢ 𝑣⸨x₁, x₂⸩ 𝑣⸨y₁, y₂⸩ x⸨⸩.x₁⟦⟧.𝟘 |ₚ y⸨⸩.y₁⟦⟧.𝟘 |ₚ x₂⸨⸩.y₂⸨⸩.z⟦⟧.𝟘 ∷
+    x ∶ ⊥‚ y ∶ ⊥‚ z ∶ 𝟙 := by
+  apply Typing.cut ∅ _ _ _ _ _ (𝟙)
+  rw [HyperEnv.merge_unitL, Env.merge_comm]
+  conv => lhs ; rhs ; rhs ; rw [Env.merge_assoc]
+  apply Typing.cut _ _ _ _ _ _ (𝟙)
+  apply Typing.mix
+  · apply Typing.bot
+    apply Typing.one
+    exact Typing.mix₀
+  · apply Typing.mix
+    · rw [Env.merge_comm]
+      apply Typing.bot
+      apply Typing.one
+      exact Typing.mix₀
+    · conv => lhs ; rhs ; rw [Env.merge_comm, ←Env.merge_assoc] ; lhs ; rw [Env.merge_comm]
+      apply Typing.bot
+      apply Typing.bot
+      apply Typing.one
+      exact Typing.mix₀
+
+
+example (𝒢 : HyperEnv) (Δ Γ Ξ : Env) (x y x' y' : PName) (P' : Proc) (B : Types) :
+  Typing ((𝒢 |ₕ {Γ‚ x ∶ B}) |ₕ {Δ‚ Ξ‚ y ∶ Bᗮ}) (𝑣⸨x', y'⸩ P') =
+    Typing (𝒢 |ₕ {Γ‚ x ∶ B} |ₕ {(Δ‚ Ξ)‚ y ∶ Bᗮ}) (𝑣⸨x', y'⸩ P') := by simp
